disk-betree/ImplSync.i.dfy
@@ -90,8 +90,7 @@ module ImplSync {
       ref in IS.IIndirectionTable(s.frozenIndirectionTable.value).locs
   ensures IS.WFVars(s')
   ensures BC.Dirty(k, old(IS.IVars(s)), IS.IVars(s'), ref, IS.INode(node))
-  // NOALIAS statically enforced no-aliasing would probably help here
-  ensures s'.ephemeralIndirectionTable.Repr == s.ephemeralIndirectionTable.Repr
+  ensures s'.ephemeralIndirectionTable == s.ephemeralIndirectionTable
   // NOALIAS statically enforced no-aliasing would probably help here
   ensures forall r | r in s.ephemeralIndirectionTable.Repr :: fresh(r) || r in old(s.ephemeralIndirectionTable.Repr)
   modifies s.ephemeralIndirectionTable.Repr
@@ -308,6 +307,10 @@ module ImplSync {
   requires BBC.Inv(k, IS.IVars(s))
   ensures IS.WFVars(s')
   ensures ImplADM.M.Next(Ik(k), old(IS.IVars(s)), IS.IVars(s'), UI.NoOp, io.diskOp())
+  // NOALIAS statically enforced no-aliasing would probably help here
+  ensures s'.ephemeralIndirectionTable.Repr == s.ephemeralIndirectionTable.Repr
+  // NOALIAS statically enforced no-aliasing would probably help here
+  ensures forall r | r in s.ephemeralIndirectionTable.Repr :: fresh(r) || r in old(s.ephemeralIndirectionTable.Repr)
   modifies s.ephemeralIndirectionTable.Repr
   {
     if s.frozenIndirectionTable.Some? {
@@ -360,6 +363,8 @@ module ImplSync {
   requires BBC.Inv(k, IS.IVars(s))
   ensures IS.WFVars(s')
   ensures ImplADM.M.Next(Ik(k), old(IS.IVars(s)), IS.IVars(s'), UI.NoOp, io.diskOp())
+  // NOALIAS statically enforced no-aliasing would probably help here
+  ensures forall r | r in s.ephemeralIndirectionTable.Repr :: fresh(r) || r in old(s.ephemeralIndirectionTable.Repr)
   modifies s.ephemeralIndirectionTable.Repr
   {
     if (BT.G.Root() !in s.cache) {
@@ -841,6 +846,8 @@ module ImplSync {
   modifies io
   ensures IS.WFVars(s')
   ensures ImplADM.M.Next(Ik(k), old(IS.IVars(s)), IS.IVars(s'), UI.NoOp, io.diskOp())
+  // NOALIAS statically enforced no-aliasing would probably help here
+  ensures forall r | r in s.ephemeralIndirectionTable.Repr :: fresh(r) || r in old(s.ephemeralIndirectionTable.Repr)
   modifies s.ephemeralIndirectionTable.Repr
   {
     if s.frozenIndirectionTable.Some? {
@@ -1006,6 +1013,8 @@ module ImplSync {
   requires BBC.Inv(k, IS.IVars(s))
   ensures IS.WFVars(s')
   ensures ImplADM.M.Next(Ik(k), old(IS.IVars(s)), IS.IVars(s'), UI.NoOp, io.diskOp())
+  // NOALIAS statically enforced no-aliasing would probably help here
+  ensures forall r | r in s.ephemeralIndirectionTable.Repr :: fresh(r) || r in old(s.ephemeralIndirectionTable.Repr)
   modifies s.ephemeralIndirectionTable.Repr
   {
     if s.frozenIndirectionTable.Some? {
@@ -1122,6 +1131,8 @@ module ImplSync {
   modifies io
   ensures IS.WFVars(s')
   ensures ImplADM.M.Next(Ik(k), old(IS.IVars(s)), IS.IVars(s'), UI.NoOp, io.diskOp())
+  // NOALIAS statically enforced no-aliasing would probably help here
+  ensures forall r | r in s.ephemeralIndirectionTable.Repr :: fresh(r) || r in old(s.ephemeralIndirectionTable.Repr)
   modifies s.ephemeralIndirectionTable.Repr
   {
     if (ref !in s.cache) {
@@ -1152,6 +1163,7 @@ module ImplSync {
       if (node.children.Some?) {
         // internal node case: flush
         s' := flush(k, s, io, ref, i);
+        return;
       } else {
         // leaf case
 
@@ -1195,11 +1207,12 @@ module ImplSync {
 
         //assert BT.ValidRepivot(BT.Repivot(ref, node, pivots));
         ghost var step := BT.BetreeRepivot(BT.Repivot(ref, IS.INode(node), pivots));
-        assume BT.ValidBetreeStep(step);
-        assume |BT.BetreeStepOps(step)| == 1; // TODO
-        assume BC.OpStep(k, old(IS.IVars(s)), IS.IVars(s'), BT.BetreeStepOps(step)[0]);
+        assert BT.ValidBetreeStep(step);
+        assert |BT.BetreeStepOps(step)| == 1; // TODO
+        assert BC.OpStep(k, old(IS.IVars(s)), IS.IVars(s'), BT.BetreeStepOps(step)[0]);
         BC.MakeTransaction1(k, old(IS.IVars(s)), IS.IVars(s'), BT.BetreeStepOps(step));
-        assume stepsBetree(k, old(IS.IVars(s)), IS.IVars(s'), UI.NoOp, step);
+        assert stepsBetree(k, old(IS.IVars(s)), IS.IVars(s'), UI.NoOp, step);
+        return;
       }
     } else if |node.buckets| > Marshalling.CapNumBuckets() as int {
       if (parentref !in s.cache) {
@@ -1215,10 +1228,12 @@ module ImplSync {
       var i :| 0 <= i < |parent.children.value| && parent.children.value[i] == ref;
 
       s' := doSplit(k, s, io, parentref, ref, i);
+      return;
     } else {
       s' := s;
       assert noop(k, old(IS.IVars(s)), IS.IVars(s'));
       print "giving up; fixBigNode\n";
+      return;
     }
   }
 
@@ -1285,8 +1300,10 @@ module ImplSync {
 
   method AssignRefToLBA(table: IS.MutIndirectionTable, ref: IS.Reference, loc: BC.Location)
   requires table.Inv()
-  ensures IS.IIndirectionTable(table) ==
-      old(BC.assignRefToLocation(IS.IIndirectionTable(table), ref, loc))
+  ensures table.Inv()
+  ensures IS.IIndirectionTable(table) == old(BC.assignRefToLocation(IS.IIndirectionTable(table), ref, loc))
+  // NOALIAS statically enforced no-aliasing would probably help here
+  ensures forall r | r in table.Repr :: fresh(r) || r in old(table.Repr)
   modifies table.Repr
   {
     var locGraph := table.Remove(ref);
@@ -1295,24 +1312,29 @@ module ImplSync {
       assume table.Count as nat < 0x10000000000000000 / 8;
       var _ := table.Insert(ref, (Some(loc), graph));
     }
-    assume IS.IIndirectionTable(table) ==
+    assert IS.IIndirectionTable(table) ==
         old(BC.assignRefToLocation(IS.IIndirectionTable(table), ref, loc));
   }
 
   method FindDeallocable(s: ImplVariables) returns (ref: Option<IS.Reference>)
+  requires IS.WFVars(s)
   requires s.Ready?
-  requires s.ephemeralIndirectionTable.Inv()
   ensures ref.Some? ==> ref.value in IS.IIndirectionTable(s.ephemeralIndirectionTable).graph
   ensures ref.Some? ==> deallocable(s, ref.value)
   ensures ref.None? ==> forall r | r in IS.IIndirectionTable(s.ephemeralIndirectionTable).graph :: !deallocable(s, r)
   {
     // TODO once we have an lba freelist, rewrite this to avoid extracting a `map` from `s.ephemeralIndirectionTable`
     var ephemeralTable := s.ephemeralIndirectionTable.ToMap();
-    var ephemeralRefs := SetToSeq(set k | k in ephemeralTable);
+    var ephemeralRefs := SetToSeq(ephemeralTable.Keys);
+
     assume |ephemeralRefs| < 0x1_0000_0000_0000_0000;
+
     var i: uint64 := 0;
     while i as int < |ephemeralRefs|
     invariant i as int <= |ephemeralRefs|
+    invariant forall k : nat | k < i as nat :: (
+        && ephemeralRefs[k] in IS.IIndirectionTable(s.ephemeralIndirectionTable).graph
+        && !deallocable(s, ephemeralRefs[k]))
     {
       var ref := ephemeralRefs[i];
       var isDeallocable := Deallocable(s, ref);
@@ -1321,7 +1343,7 @@ module ImplSync {
       }
       i := i + 1;
     }
-    assume forall r | r in IS.IIndirectionTable(s.ephemeralIndirectionTable).graph :: !deallocable(s, r);
+    assert forall r | r in IS.IIndirectionTable(s.ephemeralIndirectionTable).graph :: !deallocable(s, r);
     return None;
   }
 
@@ -1330,25 +1352,28 @@ module ImplSync {
   requires s.Ready?
   ensures ref.Some? ==> ref.value in IS.IIndirectionTable(s.ephemeralIndirectionTable).graph
   ensures ref.Some? ==> ref.value in s.cache && !Marshalling.CappedNode(s.cache[ref.value])
-  ensures ref.None? ==> forall r | r in IS.IIndirectionTable(s.ephemeralIndirectionTable).graph :: r in s.cache && Marshalling.CappedNode(s.cache[r])
+  ensures ref.None? ==> forall r | r in IS.IIndirectionTable(s.ephemeralIndirectionTable).graph :: r !in s.cache || Marshalling.CappedNode(s.cache[r])
   {
     // TODO once we have an lba freelist, rewrite this to avoid extracting a `map` from `s.ephemeralIndirectionTable`
     var ephemeralTable := s.ephemeralIndirectionTable.ToMap();
-    var ephemeralRefs := SetToSeq(set k | k in ephemeralTable);
+    var ephemeralRefs := SetToSeq(ephemeralTable.Keys);
+
     assume |ephemeralRefs| < 0x1_0000_0000_0000_0000;
+
     var i: uint64 := 0;
     while i as int < |ephemeralRefs|
     invariant i as int <= |ephemeralRefs|
+    invariant forall k : nat | k < i as nat :: (
+        && ephemeralRefs[k] in IS.IIndirectionTable(s.ephemeralIndirectionTable).graph
+        && (ephemeralRefs[k] !in s.cache || Marshalling.CappedNode(s.cache[ephemeralRefs[k]])))
     {
       var ref := ephemeralRefs[i];
-      assume ref in s.cache;
-      if !Marshalling.CappedNode(s.cache[ref]) {
-        assume ref in IS.IIndirectionTable(s.ephemeralIndirectionTable).graph;
+      if ref in s.cache && !Marshalling.CappedNode(s.cache[ref]) {
         return Some(ref);
       }
       i := i + 1;
     }
-    assume forall r | r in IS.IIndirectionTable(s.ephemeralIndirectionTable).graph :: r in s.cache && Marshalling.CappedNode(s.cache[r]);
+    assert forall r | r in IS.IIndirectionTable(s.ephemeralIndirectionTable).graph :: r !in s.cache || Marshalling.CappedNode(s.cache[r]);
     return None;
   }
 
@@ -1363,22 +1388,27 @@ module ImplSync {
   {
     // TODO once we have an lba freelist, rewrite this to avoid extracting a `map` from `s.ephemeralIndirectionTable`
     var frozenTable := s.frozenIndirectionTable.value.ToMap();
-    var frozenRefs := SetToSeq(set k | k in frozenTable);
+    var frozenRefs := SetToSeq(frozenTable.Keys);
+
     assume |frozenRefs| < 0x1_0000_0000_0000_0000;
+
     var i: uint64 := 0;
     while i as int < |frozenRefs|
     invariant i as int <= |frozenRefs|
+    invariant forall k : nat | k < i as nat :: (
+        && frozenRefs[k] in IS.IIndirectionTable(s.frozenIndirectionTable.value).graph
+        && frozenRefs[k] in IS.IIndirectionTable(s.frozenIndirectionTable.value).locs)
     {
       var ref := frozenRefs[i];
       var lbaGraph := s.frozenIndirectionTable.value.Get(ref);
-      assume lbaGraph.Some?;
+      assert lbaGraph.Some?;
       var (lba, _) := lbaGraph.value;
       if lba.None? {
         return Some(ref);
       }
       i := i + 1;
     }
-    assume forall r | r in IS.IIndirectionTable(s.frozenIndirectionTable.value).graph
+    assert forall r | r in IS.IIndirectionTable(s.frozenIndirectionTable.value).graph
         :: r in IS.IIndirectionTable(s.frozenIndirectionTable.value).locs;
     return None;
   }
@@ -1395,7 +1425,7 @@ module ImplSync {
     var ephemeralTable := s.ephemeralIndirectionTable.ToMap();
 
     var ephemeralRefs := SetToSeq(ephemeralTable.Keys);
-    assert forall k | k in ephemeralRefs :: k in ephemeralTable; // TODO
+    assert forall k | k in ephemeralRefs :: k in ephemeralTable;
 
     assert forall k | k in ephemeralRefs :: k in IS.IIndirectionTable(s.ephemeralIndirectionTable).graph; // TODO
 
@@ -1427,6 +1457,151 @@ module ImplSync {
     assert false;
   }
 
+  method {:fuel BC.GraphClosed,0} syncNotFrozen(k: ImplConstants, s: ImplVariables, io: DiskIOHandler)
+  returns (s': ImplVariables)
+  requires io.initialized()
+  modifies io
+  requires IS.WFVars(s)
+  requires BBC.Inv(k, IS.IVars(s))
+  requires s.Ready?
+  requires s.outstandingIndirectionTableWrite.None?
+  requires s.rootBucket == TTT.EmptyTree
+  requires s.frozenIndirectionTable.None?
+  ensures IS.WFVars(s')
+  ensures ImplADM.M.Next(Ik(k), old(IS.IVars(s)), IS.IVars(s'), UI.NoOp, io.diskOp())
+  // NOALIAS statically enforced no-aliasing would probably help here
+  ensures s.Ready? ==> forall r | r in s.ephemeralIndirectionTable.Repr :: fresh(r) || r in old(s.ephemeralIndirectionTable.Repr)
+  modifies if s.Ready? then s.ephemeralIndirectionTable.Repr else {}
+  {
+    var ephemeralTable := s.ephemeralIndirectionTable.ToMap();
+    var ephemeralGraph := map k | k in ephemeralTable :: ephemeralTable[k].1;
+    var foundDeallocable := FindDeallocable(s);
+    if foundDeallocable.Some? {
+      s' := Dealloc(k, s, io, foundDeallocable.value);
+      return;
+    }
+    var foundUncapped := FindUncappedNodeInCache(s);
+    if foundUncapped.Some? {
+      var ref := foundUncapped.value;
+      assert ref in IS.IIndirectionTable(s.ephemeralIndirectionTable).graph;
+      assert ref in s.cache && !Marshalling.CappedNode(s.cache[foundUncapped.value]);
+      if (ref == BT.G.Root()) {
+        s' := fixBigRoot(k, s, io);
+        return;
+      } else {
+        assert !deallocable(s, ref);
+        assert !(forall r | r in IS.IIndirectionTable(s.ephemeralIndirectionTable).graph ::
+            ref !in IS.IIndirectionTable(s.ephemeralIndirectionTable).graph[r]);
+        assert !(forall r :: r in IS.IIndirectionTable(s.ephemeralIndirectionTable).graph ==>
+            ref !in IS.IIndirectionTable(s.ephemeralIndirectionTable).graph[r]);
+        assert (exists r :: !(r in IS.IIndirectionTable(s.ephemeralIndirectionTable).graph ==>
+            ref !in IS.IIndirectionTable(s.ephemeralIndirectionTable).graph[r]));
+        var r := FindRefNotPointingToRefInEphemeral(s, ref);
+        assert !(r in IS.IIndirectionTable(s.ephemeralIndirectionTable).graph ==>
+            ref !in IS.IIndirectionTable(s.ephemeralIndirectionTable).graph[r]);
+        s' := fixBigNode(k, s, io, ref, r);
+        return;
+      }
+    } else {
+      var clonedEphemeralIndirectionTable := s.ephemeralIndirectionTable.Clone();
+      s' := s.(frozenIndirectionTable := Some(clonedEphemeralIndirectionTable))
+          .(syncReqs := BC.syncReqs3to2(s.syncReqs));
+
+      // TODO
+      assume IS.IVars(s') == old(IS.IVars(s))
+          .(frozenIndirectionTable := Some(old(IS.IVars(s)).ephemeralIndirectionTable))
+          .(syncReqs := BC.syncReqs3to2(old(IS.IVars(s)).syncReqs));
+
+      assert BC.Freeze(Ik(k), old(IS.IVars(s)), IS.IVars(s'), ImplADM.M.IDiskOp(io.diskOp()));
+      assert BBC.BlockCacheMove(Ik(k), old(IS.IVars(s)), IS.IVars(s'), UI.NoOp, ImplADM.M.IDiskOp(io.diskOp()), BC.FreezeStep);
+      assert stepsBC(k, old(IS.IVars(s)), IS.IVars(s'), UI.NoOp, io, BC.FreezeStep);
+      return;
+    }
+  }
+
+  method {:fuel BC.GraphClosed,0} syncFoundInFrozen(k: ImplConstants, s: ImplVariables, io: DiskIOHandler, ref: IS.Reference)
+  returns (s': ImplVariables)
+  requires io.initialized()
+  modifies io
+  requires IS.WFVars(s)
+  requires BBC.Inv(k, IS.IVars(s))
+  requires s.Ready?
+  requires s.outstandingIndirectionTableWrite.None?
+  requires s.rootBucket == TTT.EmptyTree
+  requires s.frozenIndirectionTable.Some?
+  requires ref in IS.IIndirectionTable(s.frozenIndirectionTable.value).graph 
+  requires ref !in IS.IIndirectionTable(s.frozenIndirectionTable.value).locs
+  ensures IS.WFVars(s')
+  ensures ImplADM.M.Next(Ik(k), old(IS.IVars(s)), IS.IVars(s'), UI.NoOp, io.diskOp())
+  // NOALIAS statically enforced no-aliasing would probably help here
+  ensures s.Ready? ==> forall r | r in s.ephemeralIndirectionTable.Repr :: fresh(r) || r in old(s.ephemeralIndirectionTable.Repr)
+  modifies if s.Ready? then s.ephemeralIndirectionTable.Repr else {}
+  modifies if s.Ready? then s.frozenIndirectionTable.value.Repr else {}
+  {
+    assert ref in IS.IIndirectionTable(s.frozenIndirectionTable.value).graph;
+    assert ref !in IS.IIndirectionTable(s.frozenIndirectionTable.value).locs;
+
+    if (!Marshalling.CappedNode(s.cache[ref])) {
+      // TODO we should be able to prove this is impossible by adding an invariant
+      // about frozenIndirectionTable (that is, we should never be freezing a table
+      // with too-big nodes in it)
+      s' := s;
+      assert noop(k, old(IS.IVars(s)), IS.IVars(s'));
+      print "sync: giving up; frozen table has big node rip (TODO we should prove this case impossible)\n";
+      return;
+    }
+
+    var ephemeralRef := s.ephemeralIndirectionTable.Get(ref);
+    if ephemeralRef.Some? && ephemeralRef.value.0.Some? {
+      assert ref in IS.IIndirectionTable(s.ephemeralIndirectionTable).locs;
+      // TODO we should be able to prove this is impossible as well
+      s' := s;
+      assert noop(k, old(IS.IVars(s)), IS.IVars(s'));
+      print "sync: giving up; ref already in ephemeralIndirectionTable.locs but not frozen";
+      return;
+    }
+
+    assert ref !in IS.IIndirectionTable(s.ephemeralIndirectionTable).locs;
+
+    INodeRootEqINodeForEmptyRootBucket(s.cache[ref]);
+    var id, loc := FindLocationAndRequestWrite(s, io, IS.SectorBlock(s.cache[ref]));
+    if (id.Some?) {
+      AssignRefToLBA(s.ephemeralIndirectionTable, ref, loc.value);
+      assert IS.IIndirectionTable(s.ephemeralIndirectionTable) ==
+        BC.assignRefToLocation(IS.IIndirectionTable(s.ephemeralIndirectionTable), ref, loc.value);
+      AssignRefToLBA(s.frozenIndirectionTable.value, ref, loc.value);
+      assert IS.IIndirectionTable(s.frozenIndirectionTable.value) ==
+        BC.assignRefToLocation(IS.IIndirectionTable(s.frozenIndirectionTable.value), ref, loc.value);
+      s' := s
+        .(outstandingBlockWrites := s.outstandingBlockWrites[id.value := BC.OutstandingWrite(ref, loc.value)]);
+      
+      ghost var reqWriteLoc := ImplADM.M.IDiskOp(io.diskOp()).reqWrite.loc;
+
+      // TODO
+      assume reqWriteLoc.addr != BC.IndirectionTableLBA();
+      assert BC.ValidLocationForNode(reqWriteLoc);
+
+      // TODO
+      assume old(forall ref | ref in IS.IIndirectionTable(s.persistentIndirectionTable).locs ::
+          IS.IIndirectionTable(s.persistentIndirectionTable).locs[ref].addr != reqWriteLoc.addr);
+      assume old(forall ref | ref in IS.IIndirectionTable(s.ephemeralIndirectionTable).locs ::
+          IS.IIndirectionTable(s.ephemeralIndirectionTable).locs[ref].addr != reqWriteLoc.addr);
+      assume old(s.frozenIndirectionTable.Some? ==> forall ref | ref in IS.IIndirectionTable(s.frozenIndirectionTable.value).locs ::
+          IS.IIndirectionTable(s.frozenIndirectionTable.value).locs[ref].addr != reqWriteLoc.addr);
+      assume old(forall id | id in s.outstandingBlockWrites ::
+          s.outstandingBlockWrites[id].loc.addr != reqWriteLoc.addr);
+
+      assert BC.WriteBackReq(Ik(k), old(IS.IVars(s)), IS.IVars(s'), ImplADM.M.IDiskOp(io.diskOp()), ref);
+      assert stepsBC(k, old(IS.IVars(s)), IS.IVars(s'), UI.NoOp, io, BC.WriteBackReqStep(ref));
+      return;
+    } else {
+      s' := s;
+      assert noop(k, old(IS.IVars(s)), IS.IVars(s'));
+      print "sync: giving up; write req failed\n";
+      return;
+    }
+  }
+
   method {:fuel BC.GraphClosed,0} sync(k: ImplConstants, s: ImplVariables, io: DiskIOHandler)
   returns (s': ImplVariables)
   requires io.initialized()
@@ -1435,9 +1610,10 @@ module ImplSync {
   requires BBC.Inv(k, IS.IVars(s))
   ensures IS.WFVars(s')
   ensures ImplADM.M.Next(Ik(k), old(IS.IVars(s)), IS.IVars(s'), UI.NoOp, io.diskOp())
+  // NOALIAS statically enforced no-aliasing would probably help here
+  ensures s.Ready? ==> forall r | r in s.ephemeralIndirectionTable.Repr :: fresh(r) || r in old(s.ephemeralIndirectionTable.Repr)
+  modifies if s.Ready? then s.ephemeralIndirectionTable.Repr else {}
   {
-    assume false; // TODO timing out
-
     if (s.Unready?) {
       // TODO we could just do nothing here instead
       s' := PageInIndirectionTableReq(k, s, io);
@@ -1466,101 +1642,31 @@ module ImplSync {
     //    - Write the frozenIndirectionTable to disk
 
     if (s.frozenIndirectionTable.None?) {
-      var ephemeralTable := s.ephemeralIndirectionTable.ToMap();
-      var ephemeralGraph := map k | k in ephemeralTable :: ephemeralTable[k].1;
-      var foundDeallocable := FindDeallocable(s);
-      if foundDeallocable.Some? {
-        s' := Dealloc(k, s, io, foundDeallocable.value);
-        return;
-      }
-      var foundUncapped := FindUncappedNodeInCache(s);
-      if foundUncapped.Some? {
-        var ref := foundUncapped.value;
-        assert ref in IS.IIndirectionTable(s.ephemeralIndirectionTable).graph;
-        assert ref in s.cache && !Marshalling.CappedNode(s.cache[foundUncapped.value]);
-        if (ref == BT.G.Root()) {
-          s' := fixBigRoot(k, s, io);
-        } else {
-          assert !deallocable(s, ref);
-          assert !(forall r | r in IS.IIndirectionTable(s.ephemeralIndirectionTable).graph ::
-              ref !in IS.IIndirectionTable(s.ephemeralIndirectionTable).graph[r]);
-          assert !(forall r :: r in IS.IIndirectionTable(s.ephemeralIndirectionTable).graph ==>
-              ref !in IS.IIndirectionTable(s.ephemeralIndirectionTable).graph[r]);
-          assert (exists r :: !(r in IS.IIndirectionTable(s.ephemeralIndirectionTable).graph ==>
-              ref !in IS.IIndirectionTable(s.ephemeralIndirectionTable).graph[r]));
-          var r := FindRefNotPointingToRefInEphemeral(s, ref);
-          assert !(r in IS.IIndirectionTable(s.ephemeralIndirectionTable).graph ==>
-              ref !in IS.IIndirectionTable(s.ephemeralIndirectionTable).graph[r]);
-          s' := fixBigNode(k, s, io, ref, r);
-        }
-        return;
-      } else {
-        s' := s.(frozenIndirectionTable := Some(s.ephemeralIndirectionTable))
-            .(syncReqs := BC.syncReqs3to2(s.syncReqs));
-        assert BC.Freeze(Ik(k), old(IS.IVars(s)), IS.IVars(s'), ImplADM.M.IDiskOp(io.diskOp()));
-        assert stepsBC(k, IS.IVars(s), IS.IVars(s'), UI.NoOp, io, BC.FreezeStep);
-        return;
-      }
+      s' := syncNotFrozen(k, s, io);
+      return;
     }
     var foundInFrozen := FindRefInFrozenWithNoLba(s);
     if foundInFrozen.Some? {
-      var ref := foundInFrozen.value;
-      assert ref in IS.IIndirectionTable(s.frozenIndirectionTable.value).graph;
-      assert ref !in IS.IIndirectionTable(s.frozenIndirectionTable.value).locs;
-
-      if (!Marshalling.CappedNode(s.cache[ref])) {
-        // TODO we should be able to prove this is impossible by adding an invariant
-        // about frozenIndirectionTable (that is, we should never be freezing a table
-        // with too-big nodes in it)
-        s' := s;
-        assert noop(k, old(IS.IVars(s)), IS.IVars(s'));
-        print "sync: giving up; frozen table has big node rip (TODO we should prove this case impossible)\n";
-        return;
-      }
-
-      var ephemeralRef := s.ephemeralIndirectionTable.Get(ref);
-      if ephemeralRef.Some? && ephemeralRef.value.0.Some? {
-        assert ref in IS.IIndirectionTable(s.ephemeralIndirectionTable).locs;
-        // TODO we should be able to prove this is impossible as well
-        s' := s;
-        assert noop(k, old(IS.IVars(s)), IS.IVars(s'));
-        print "sync: giving up; ref already in ephemeralIndirectionTable.locs but not frozen";
-        return;
-      }
-
-      INodeRootEqINodeForEmptyRootBucket(s.cache[ref]);
-      var id, loc := FindLocationAndRequestWrite(s, io, IS.SectorBlock(s.cache[ref]));
-      if (id.Some?) {
-        AssignRefToLBA(s.ephemeralIndirectionTable, ref, loc.value);
-        assert IS.IIndirectionTable(s.ephemeralIndirectionTable) ==
-          BC.assignRefToLocation(IS.IIndirectionTable(s.ephemeralIndirectionTable), ref, loc.value);
-        AssignRefToLBA(s.frozenIndirectionTable.value, ref, loc.value);
-        assert IS.IIndirectionTable(s.frozenIndirectionTable.value) ==
-          BC.assignRefToLocation(IS.IIndirectionTable(s.frozenIndirectionTable.value), ref, loc.value);
-        s' := s
-          .(outstandingBlockWrites := s.outstandingBlockWrites[id.value := BC.OutstandingWrite(ref, loc.value)]);
-        assert BC.WriteBackReq(Ik(k), old(IS.IVars(s)), IS.IVars(s'), ImplADM.M.IDiskOp(io.diskOp()), ref);
-        assert stepsBC(k, IS.IVars(s), IS.IVars(s'), UI.NoOp, io, BC.WriteBackReqStep(ref));
-      } else {
-        s' := s;
-        assert noop(k, old(IS.IVars(s)), IS.IVars(s'));
-        print "sync: giving up; write req failed\n";
-      }
+      s' := syncFoundInFrozen(k, s, io, foundInFrozen.value);
+      return;
     } else if (s.outstandingBlockWrites != map[]) {
       s' := s;
       assert noop(k, old(IS.IVars(s)), IS.IVars(s'));
       print "sync: giving up; blocks are still being written\n";
+      return;
     } else {
       LBAType.reveal_ValidAddr();
       var id := RequestWrite(io, BC.IndirectionTableLocation(), IS.SectorIndirectionTable(s.frozenIndirectionTable.value));
       if (id.Some?) {
         s' := s.(outstandingIndirectionTableWrite := id);
         assert BC.WriteBackIndirectionTableReq(Ik(k), old(IS.IVars(s)), IS.IVars(s'), ImplADM.M.IDiskOp(io.diskOp()));
-        assert stepsBC(k, IS.IVars(s), IS.IVars(s'), UI.NoOp, io, BC.WriteBackIndirectionTableReqStep);
+        assert stepsBC(k, old(IS.IVars(s)), IS.IVars(s'), UI.NoOp, io, BC.WriteBackIndirectionTableReqStep);
+        return;
       } else {
         s' := s;
         assert noop(k, old(IS.IVars(s)), IS.IVars(s'));
         print "sync: giving up; write back indirection table failed (no id)\n";
+        return;
       }
     }
   }
